iris/TrampStepPt.v
@@ -447,7 +447,7 @@ Section TrampFetchPt.
     iPoseProof "Hhw" as "#Hhwc".
     iDestruct "Hhwc" as (misa0 mseccfg0 pmar0 elp0)
       "(#Hmisa & #Hmseccfg & #Hpma & #Hhtif & #Help & %HmisaS & %HmisaC &
-        %HmisaU & %HmisaM & %Hpma_all & %Hseccfg1 & %Hseccfg2 & %Help_np & %HmisaA & %Hmisa_val0 & %Hmseccfg_val0)".
+        %HmisaU & %HmisaM & %Hpma_all & %Hseccfg1 & %Hseccfg2 & %Help_np & %HmisaA & %Hmisa_val0 & %Hmseccfg_val0 & #Hkmapb)".
     iDestruct "Hinstr" as "[%Hnlpad Hr]".
     iDestruct "Hr" as (r) "[%Hrvc [Hbytes Hdec]]".
     iAssert (⌜ match r with F_Base _ => True | F_RVC _ => True | _ => False end ⌝)%I as %Hrok.
