iris/UserretEntryPt.v
@@ -92,7 +92,7 @@ Section UserretEntryPt.
     iPoseProof "Hhw" as "#Hhwc".
     iDestruct "Hhwc" as (misa0 mseccfg0 pmar0 elp0)
       "(#Hmisa & #Hmseccfg & #Hpma & #Hhtif & #Help & %HmisaS & %HmisaC &
-        %HmisaU & %HmisaM & %Hpma_all & %Hseccfg1 & %Hseccfg2 & %Help_np & %HmisaA & %Hmisa_val0 & %Hmseccfg_val0)".
+        %HmisaU & %HmisaM & %Hpma_all & %Hseccfg1 & %Hseccfg2 & %Help_np & %HmisaA & %Hmisa_val0 & %Hmseccfg_val0 & #Hkmapb)".
     assert (Hva01 : add_vec_int (uva 0x9c) 4 = uva 0xa0)
       by (apply bv_eq; vm_compute; reflexivity).
     assert (Hva02 : add_vec_int (uva 0xa0) 4 = uva 0xa4)
