iris/WpGprCsrwA.v
@@ -863,7 +863,7 @@ Section WpCsrwGprNewA.
     iPoseProof "Hhw" as "#Hhwc".
     iDestruct "Hhwc" as (misa0 mseccfg0 pmar0 elp0)
       "(#Hmisa & #Hmseccfg & #Hpma & #Hhtif & #Help & %HmisaS & %HmisaC &
-        %HmisaU & %HmisaM & %Hpma_all & %Hseccfg1 & %Hseccfg2 & %Help_np & %HmisaA & %Hmisa_val0 & %Hmseccfg_val0)".
+        %HmisaU & %HmisaM & %Hpma_all & %Hseccfg1 & %Hseccfg2 & %Help_np & %HmisaA & %Hmisa_val0 & %Hmseccfg_val0 & #Hkmapb)".
     iApply (wp_instr Φ pc false (CSRReg (csr_medeleg, Regidx rs1, zreg, CSRRW)) pmpcfg0
               Hpmp with "Hmm_wp Hpmpc_wp Hpc Hinstr").
     iIntros (σ Hpceq) "Hsi".
@@ -944,7 +944,7 @@ Section WpCsrwGprNewA.
     iPoseProof "Hhw" as "#Hhwc".
     iDestruct "Hhwc" as (misa0 mseccfg0 pmar0 elp0)
       "(#Hmisa & #Hmseccfg & #Hpma & #Hhtif & #Help & %HmisaS & %HmisaC &
-        %HmisaU & %HmisaM & %Hpma_all & %Hseccfg1 & %Hseccfg2 & %Help_np & %HmisaA & %Hmisa_val0 & %Hmseccfg_val0)".
+        %HmisaU & %HmisaM & %Hpma_all & %Hseccfg1 & %Hseccfg2 & %Help_np & %HmisaA & %Hmisa_val0 & %Hmseccfg_val0 & #Hkmapb)".
     iApply (wp_instr Φ pc false (CSRReg (csr_mcounteren, Regidx rs1, zreg, CSRRW)) pmpcfg0
               Hpmp with "Hmm_wp Hpmpc_wp Hpc Hinstr").
     iIntros (σ Hpceq) "Hsi".
@@ -1023,7 +1023,7 @@ Section WpCsrwGprNewA.
     iPoseProof "Hhw" as "#Hhwc".
     iDestruct "Hhwc" as (misa0 mseccfg0 pmar0 elp0)
       "(#Hmisa & #Hmseccfg & #Hpma & #Hhtif & #Help & %HmisaS & %HmisaC &
-        %HmisaU & %HmisaM & %Hpma_all & %Hseccfg1 & %Hseccfg2 & %Help_np & %HmisaA & %Hmisa_val0 & %Hmseccfg_val0)".
+        %HmisaU & %HmisaM & %Hpma_all & %Hseccfg1 & %Hseccfg2 & %Help_np & %HmisaA & %Hmisa_val0 & %Hmseccfg_val0 & #Hkmapb)".
     iApply (wp_instr Φ pc false (CSRReg (csr_menvcfg, Regidx rs1, zreg, CSRRW)) pmpcfg0
               Hpmp with "Hmm_wp Hpmpc_wp Hpc Hinstr").
     iIntros (σ Hpceq) "Hsi".
@@ -1103,7 +1103,7 @@ Section WpCsrwGprNewA.
     iPoseProof "Hhw" as "#Hhwc".
     iDestruct "Hhwc" as (misa0 mseccfg0 pmar0 elp0)
       "(#Hmisa & #Hmseccfg & #Hpma & #Hhtif & #Help & %HmisaS & %HmisaC &
-        %HmisaU & %HmisaM & %Hpma_all & %Hseccfg1 & %Hseccfg2 & %Help_np & %HmisaA & %Hmisa_val0 & %Hmseccfg_val0)".
+        %HmisaU & %HmisaM & %Hpma_all & %Hseccfg1 & %Hseccfg2 & %Help_np & %HmisaA & %Hmisa_val0 & %Hmseccfg_val0 & #Hkmapb)".
     iApply (wp_instr Φ pc false (CSRReg (csr_mepc, Regidx rs1, zreg, CSRRW)) pmpcfg0
               Hpmp with "Hmm_wp Hpmpc_wp Hpc Hinstr").
     iIntros (σ Hpceq) "Hsi".
