iris/WpMmodeJalr.v
@@ -56,7 +56,7 @@ Section RvcRet.
     iPoseProof "Hhw" as "#Hhwc".
     iDestruct "Hhwc" as (misa0 mseccfg0 pmar0 elp0)
       "(#Hmisa & #Hmseccfg & #Hpma & #Hhtif & #Help & %HmisaS & %HmisaC &
-        %HmisaU & %HmisaM & %Hpma_all & %Hseccfg1 & %Hmlpe & %Help_np & %HmisaA & %Hmisa_val0 & %Hmseccfg_val0)".
+        %HmisaU & %HmisaM & %Hpma_all & %Hseccfg1 & %Hmlpe & %Help_np & %HmisaA & %Hmisa_val0 & %Hmseccfg_val0 & #Hkmapb)".
     iDestruct "Hpmpc" as "[Hpmpc_wp Hpmpc_k]".
     iApply (wp_instr Φ pc true (JALR (zeros' 12, Regidx ra, zreg)) pmpcfg0
               Hpmp with "Hmm_wp Hpmpc_wp Hpc Hinstr").
