iris/WpMmodeLoad.v
@@ -59,7 +59,7 @@ Section WpLdGpr.
     iPoseProof "Hhw" as "#Hhwc".
     iDestruct "Hhwc" as (misa0 mseccfg0 pmar0 elp0)
       "(#Hmisa & #Hmseccfg & #Hpma & #Hhtif & #Help & %HmisaS & %HmisaC &
-        %HmisaU & %HmisaM & %Hpma_all & %Hseccfg1 & %Hseccfg2 & %Help_np & %HmisaA & %Hmisa_val0 & %Hmseccfg_val0)".
+        %HmisaU & %HmisaM & %Hpma_all & %Hseccfg1 & %Hseccfg2 & %Help_np & %HmisaA & %Hmisa_val0 & %Hmseccfg_val0 & #Hkmapb)".
     destruct (Hpma_all ea 8) as (region & Hmatch & _ & Hread & _).
     iApply (wp_instr Φ pc is_rvc (LOAD (imm, Regidx rs1, Regidx rd, false, 8)) pmpcfg0
  (pmp_all_off_allows_all _ Hpmp) with "Hmm_wp Hpmpc_wp Hpc Hinstr").
@@ -223,7 +223,7 @@ Section MmodeLoadTor.
     iPoseProof "Hhw" as "#Hhwc".
     iDestruct "Hhwc" as (misa0 mseccfg0 pmar0 elp0)
       "(#Hmisa & #Hmseccfg & #Hpma & #Hhtif & #Help & %HmisaS & %HmisaC &
-        %HmisaU & %HmisaM & %Hpma_all & %Hseccfg1 & %Hseccfg2 & %Help_np & %HmisaA & %Hmisa_val0 & %Hmseccfg_val0)".
+        %HmisaU & %HmisaM & %Hpma_all & %Hseccfg1 & %Hseccfg2 & %Help_np & %HmisaA & %Hmisa_val0 & %Hmseccfg_val0 & #Hkmapb)".
     destruct (Hpma_all ea 8) as (region & Hmatch & _ & Hread & _).
     iApply (wp_instr Φ pc is_rvc (LOAD (imm, Regidx rs1, Regidx rd, false, 8)) pmpcfg0
               Hpmp with "Hmm_wp Hpmpc_wp Hpc Hinstr").
