iris/WpMmodeMret.v
@@ -70,7 +70,7 @@ Section WpMretGpr.
     iPoseProof "Hhw" as "#Hhwc".
     iDestruct "Hhwc" as (misa0 mseccfg0 pmar0 elp0)
       "(#Hmisa & #Hmseccfg & #Hpma & #Hhtif & #Help & %HmisaS & %HmisaC &
-        %HmisaU & %HmisaM & %Hpma_all & %Hseccfg1 & %Hseccfg2 & %Help_np & %HmisaA & %Hmisa_val0 & %Hmseccfg_val0)".
+        %HmisaU & %HmisaM & %Hpma_all & %Hseccfg1 & %Hseccfg2 & %Help_np & %HmisaA & %Hmisa_val0 & %Hmseccfg_val0 & #Hkmapb)".
     iDestruct "Hsi" as "[Hreg Hmem]".
     iDestruct (reg_valid    with "Hreg Hpriv")  as %Lpriv.
     iDestruct (reg_valid_dq with "Hreg Hmisa")  as %Lmisa.
