iris/WpMmodeStore.v
@@ -62,7 +62,7 @@ Section WpStoreGpr.
     iPoseProof "Hhw" as "#Hhwc".
     iDestruct "Hhwc" as (misa0 mseccfg0 pmar0 elp0)
       "(#Hmisa & #Hmseccfg & #Hpma & #Hhtif & #Help & %HmisaS & %HmisaC &
-        %HmisaU & %HmisaM & %Hpma_all & %Hseccfg1 & %Hseccfg2 & %Help_np & %HmisaA & %Hmisa_val0 & %Hmseccfg_val0)".
+        %HmisaU & %HmisaM & %Hpma_all & %Hseccfg1 & %Hseccfg2 & %Help_np & %HmisaA & %Hmisa_val0 & %Hmseccfg_val0 & #Hkmapb)".
     destruct (Hpma_all ea 8) as (region & Hmatch & _ & _ & Hwrite & _).
     iApply (wp_instr Φ pc is_rvc (STORE (imm, Regidx rs2, Regidx rs1, 8)) pmpcfg0
  (pmp_all_off_allows_all _ Hpmp) with "Hmm_wp Hpmpc_wp Hpc Hinstr").
@@ -203,7 +203,7 @@ Section MmodeStoreTor.
     iPoseProof "Hhw" as "#Hhwc".
     iDestruct "Hhwc" as (misa0 mseccfg0 pmar0 elp0)
       "(#Hmisa & #Hmseccfg & #Hpma & #Hhtif & #Help & %HmisaS & %HmisaC &
-        %HmisaU & %HmisaM & %Hpma_all & %Hseccfg1 & %Hseccfg2 & %Help_np & %HmisaA & %Hmisa_val0 & %Hmseccfg_val0)".
+        %HmisaU & %HmisaM & %Hpma_all & %Hseccfg1 & %Hseccfg2 & %Help_np & %HmisaA & %Hmisa_val0 & %Hmseccfg_val0 & #Hkmapb)".
     destruct (Hpma_all ea 8) as (region & Hmatch & _ & _ & Hwrite & _).
     iApply (wp_instr Φ pc is_rvc (STORE (imm, Regidx rs2, Regidx rs1, 8)) pmpcfg0
               Hpmp with "Hmm_wp Hpmpc_wp Hpc Hinstr").
