iris/WpSconfBtype.v
@@ -431,7 +431,7 @@ Section WpSconfBtype.
     iPoseProof "Hhw" as "#Hhwc".
     iDestruct "Hhwc" as (misa0 mseccfg0 pmar0 elp0)
       "(#Hmisa & #Hmseccfg & #Hpma & #Hhtif & #Help & %HmisaS & %HmisaC &
-        %HmisaU & %HmisaM & %Hpma_all & %Hseccfg1 & %Hseccfg2 & %Help_np & %HmisaA & %Hmisa_val0 & %Hmseccfg_val0)".
+        %HmisaU & %HmisaM & %Hpma_all & %Hseccfg1 & %Hseccfg2 & %Help_np & %HmisaA & %Hmisa_val0 & %Hmseccfg_val0 & #Hkmapb)".
     iDestruct (reg_valid_dq with "Hreg Hmisa") as %Lmisa.
     iMod (reg_update _ nextPC _ (add_vec_int pc 4) with "Hreg Hnpc") as "[Hreg Hnpc]".
     set (s_pc := set_reg σ nextPC (add_vec_int pc 4)).
@@ -491,7 +491,7 @@ Section WpSconfBtype.
     iPoseProof "Hhw" as "#Hhwc".
     iDestruct "Hhwc" as (misa0 mseccfg0 pmar0 elp0)
       "(#Hmisa & #Hmseccfg & #Hpma & #Hhtif & #Help & %HmisaS & %HmisaC &
-        %HmisaU & %HmisaM & %Hpma_all & %Hseccfg1 & %Hseccfg2 & %Help_np & %HmisaA & %Hmisa_val0 & %Hmseccfg_val0)".
+        %HmisaU & %HmisaM & %Hpma_all & %Hseccfg1 & %Hseccfg2 & %Help_np & %HmisaA & %Hmisa_val0 & %Hmseccfg_val0 & #Hkmapb)".
     iDestruct (reg_valid_dq with "Hreg Hmisa") as %Lmisa.
     iMod (reg_update _ nextPC _ (add_vec_int pc 4) with "Hreg Hnpc") as "[Hreg Hnpc]".
     set (s_pc := set_reg σ nextPC (add_vec_int pc 4)).
@@ -678,7 +678,7 @@ Section WpSconfBtype.
     iPoseProof "Hhw" as "#Hhwc".
     iDestruct "Hhwc" as (misa0 mseccfg0 pmar0 elp0)
       "(#Hmisa & #Hmseccfg & #Hpma & #Hhtif & #Help & %HmisaS & %HmisaC &
-        %HmisaU & %HmisaM & %Hpma_all & %Hseccfg1 & %Hseccfg2 & %Help_np & %HmisaA & %Hmisa_val0 & %Hmseccfg_val0)".
+        %HmisaU & %HmisaM & %Hpma_all & %Hseccfg1 & %Hseccfg2 & %Help_np & %HmisaA & %Hmisa_val0 & %Hmseccfg_val0 & #Hkmapb)".
     iDestruct (reg_valid_dq with "Hreg Hmisa") as %Lmisa.
     iMod (reg_update _ nextPC _ (add_vec_int pc 4) with "Hreg Hnpc") as "[Hreg Hnpc]".
     set (s_pc := set_reg σ nextPC (add_vec_int pc 4)).
@@ -737,7 +737,7 @@ Section WpSconfBtype.
     iPoseProof "Hhw" as "#Hhwc".
     iDestruct "Hhwc" as (misa0 mseccfg0 pmar0 elp0)
       "(#Hmisa & #Hmseccfg & #Hpma & #Hhtif & #Help & %HmisaS & %HmisaC &
-        %HmisaU & %HmisaM & %Hpma_all & %Hseccfg1 & %Hseccfg2 & %Help_np & %HmisaA & %Hmisa_val0 & %Hmseccfg_val0)".
+        %HmisaU & %HmisaM & %Hpma_all & %Hseccfg1 & %Hseccfg2 & %Help_np & %HmisaA & %Hmisa_val0 & %Hmseccfg_val0 & #Hkmapb)".
     iDestruct (reg_valid_dq with "Hreg Hmisa") as %Lmisa.
     iMod (reg_update _ nextPC _ (add_vec_int pc 4) with "Hreg Hnpc") as "[Hreg Hnpc]".
     set (s_pc := set_reg σ nextPC (add_vec_int pc 4)).
@@ -799,7 +799,7 @@ Section WpSconfBtype.
     iPoseProof "Hhw" as "#Hhwc".
     iDestruct "Hhwc" as (misa0 mseccfg0 pmar0 elp0)
       "(#Hmisa & #Hmseccfg & #Hpma & #Hhtif & #Help & %HmisaS & %HmisaC &
-        %HmisaU & %HmisaM & %Hpma_all & %Hseccfg1 & %Hseccfg2 & %Help_np & %HmisaA & %Hmisa_val0 & %Hmseccfg_val0)".
+        %HmisaU & %HmisaM & %Hpma_all & %Hseccfg1 & %Hseccfg2 & %Help_np & %HmisaA & %Hmisa_val0 & %Hmseccfg_val0 & #Hkmapb)".
     iDestruct (reg_valid_dq with "Hreg Hmisa") as %Lmisa.
     iMod (reg_update _ nextPC _ (add_vec_int pc 2) with "Hreg Hnpc") as "[Hreg Hnpc]".
     set (s_pc := set_reg σ nextPC (add_vec_int pc 2)).
@@ -862,7 +862,7 @@ Section WpSconfBtype.
     iPoseProof "Hhw" as "#Hhwc".
     iDestruct "Hhwc" as (misa0 mseccfg0 pmar0 elp0)
       "(#Hmisa & #Hmseccfg & #Hpma & #Hhtif & #Help & %HmisaS & %HmisaC &
-        %HmisaU & %HmisaM & %Hpma_all & %Hseccfg1 & %Hseccfg2 & %Help_np & %HmisaA & %Hmisa_val0 & %Hmseccfg_val0)".
+        %HmisaU & %HmisaM & %Hpma_all & %Hseccfg1 & %Hseccfg2 & %Help_np & %HmisaA & %Hmisa_val0 & %Hmseccfg_val0 & #Hkmapb)".
     iDestruct (reg_valid_dq with "Hreg Hmisa") as %Lmisa.
     iMod (reg_update _ nextPC _ (add_vec_int pc 2) with "Hreg Hnpc") as "[Hreg Hnpc]".
     set (s_pc := set_reg σ nextPC (add_vec_int pc 2)).
