iris/WpSconfCsr.v
@@ -85,7 +85,7 @@ Section WpSconfCsr.
     iPoseProof "Hhw" as "#Hhwc".
     iDestruct "Hhwc" as (misa0 mseccfg0 pmar0 elp0)
       "(#Hmisa & #Hmseccfg & #Hpma & #Hhtif & #Help & %HmisaS & %HmisaC & %HmisaU & %HmisaM &
-        %Hpma_all & %Hseccfg1 & %Hseccfg2 & %Help_np & %HmisaA & %Hmisa_val0 & %Hmseccfg_val0)".
+        %Hpma_all & %Hseccfg1 & %Hseccfg2 & %Help_np & %HmisaA & %Hmisa_val0 & %Hmseccfg_val0 & #Hkmapb)".
     iDestruct (reg_valid    with "Hreg Hpriv") as %Lpriv.
     iDestruct (reg_valid    with "Hreg Hms") as %Lms.
     iDestruct (reg_valid_dq with "Hreg Hmisa") as %Lmisa.
@@ -263,7 +263,7 @@ Section WpSconfCsr.
     iPoseProof "Hhw" as "#Hhwc".
     iDestruct "Hhwc" as (misa0 mseccfg0 pmar0 elp0)
       "(#Hmisa & #Hmseccfg & #Hpma & #Hhtif & #Help & %HmisaS & %HmisaC & %HmisaU & %HmisaM &
-        %Hpma_all & %Hseccfg1 & %Hseccfg2 & %Help_np & %HmisaA & %Hmisa_val0 & %Hmseccfg_val0)".
+        %Hpma_all & %Hseccfg1 & %Hseccfg2 & %Help_np & %HmisaA & %Hmisa_val0 & %Hmseccfg_val0 & #Hkmapb)".
     iDestruct (reg_valid    with "Hreg Hpriv") as %Lpriv.
     iDestruct (reg_valid    with "Hreg Hms") as %Lms.
     iDestruct (reg_valid_dq with "Hreg Hmisa") as %Lmisa.
@@ -495,7 +495,7 @@ Section WpSconfCsr.
     iPoseProof "Hhw" as "#Hhwc".
     iDestruct "Hhwc" as (misa0 mseccfg0 pmar0 elp0)
       "(#Hmisa & #Hmseccfg & #Hpma & #Hhtif & #Help & %HmisaS & %HmisaC & %HmisaU & %HmisaM &
-        %Hpma_all & %Hseccfg1 & %Hseccfg2 & %Help_np & %HmisaA & %Hmisa_val0 & %Hmseccfg_val0)".
+        %Hpma_all & %Hseccfg1 & %Hseccfg2 & %Help_np & %HmisaA & %Hmisa_val0 & %Hmseccfg_val0 & #Hkmapb)".
     iDestruct (reg_valid    with "Hreg Hpriv") as %Lpriv.
     iDestruct (reg_valid    with "Hreg Hms") as %Lms.
     iDestruct (reg_valid_dq with "Hreg Hmisa") as %Lmisa.
