iris/WpSconfLock.v
@@ -103,7 +103,7 @@ Section WpSconfLock.
     iPoseProof "Hhw" as "#Hhwc".
     iDestruct "Hhwc" as (misa0 mseccfg0 pmar0 elp0)
       "(#Hmisa & #Hmseccfg & #Hpma & #Hhtif & #Help & %HmisaS & %HmisaC &
-        %HmisaU & %HmisaM & %Hpma_all & %Hseccfg1 & %Hseccfg2 & %Help_np & %HmisaA & %Hmisa_val0 & %Hmseccfg_val0)".
+        %HmisaU & %HmisaM & %Hpma_all & %Hseccfg1 & %Hseccfg2 & %Help_np & %HmisaA & %Hmisa_val0 & %Hmseccfg_val0 & #Hkmapb)".
     destruct (Hpma_all pa 4) as (region_ld & Hmatch_ld0 & _ & Hread_ld & _).
     iDestruct "Hsi" as "[Hreg [Hmem Hdev]]".
     iMod (inv_acc (⊤ ∖ ↑minstretN) lockN with "Hlkinv") as "[Hbody Hclose]";
@@ -308,7 +308,7 @@ Section WpSconfLock.
     iPoseProof "Hhw" as "#Hhwc".
     iDestruct "Hhwc" as (misa0 mseccfg0 pmar0 elp0)
       "(#Hmisa & #Hmseccfg & #Hpma & #Hhtif & #Help & %HmisaS & %HmisaC &
-        %HmisaU & %HmisaM & %Hpma_all & %Hseccfg1 & %Hseccfg2 & %Help_np & %HmisaA & %Hmisa_val0 & %Hmseccfg_val0)".
+        %HmisaU & %HmisaM & %Hpma_all & %Hseccfg1 & %Hseccfg2 & %Help_np & %HmisaA & %Hmisa_val0 & %Hmseccfg_val0 & #Hkmapb)".
     destruct (Hpma_all pa 4) as (region_ld & Hmatch_ld0 & _ & Hread_ld & _).
     iDestruct "Hsi" as "[Hreg [Hmem Hdev]]".
     iMod (inv_acc (⊤ ∖ ↑minstretN) lockN with "Hlkinv") as "[Hbody Hclose]";
@@ -514,7 +514,7 @@ Section WpSconfLock.
     iPoseProof "Hhw" as "#Hhwc".
     iDestruct "Hhwc" as (misa0 mseccfg0 pmar0 elp0)
       "(#Hmisa & #Hmseccfg & #Hpma & #Hhtif & #Help & %HmisaS & %HmisaC &
-        %HmisaU & %HmisaM & %Hpma_all & %Hseccfg1 & %Hseccfg2 & %Help_np & %HmisaA & %Hmisa_val0 & %Hmseccfg_val0)".
+        %HmisaU & %HmisaM & %Hpma_all & %Hseccfg1 & %Hseccfg2 & %Help_np & %HmisaA & %Hmisa_val0 & %Hmseccfg_val0 & #Hkmapb)".
     destruct (Hpma_all pa 4) as (region_st & Hmatch_st0 & _ & _ & Hwrite_st & _).
     iDestruct "Hsi" as "[Hreg [Hmem Hdev]]".
     iMod (inv_acc (⊤ ∖ ↑minstretN) lockN with "Hlkinv") as "[Hbody Hclose]";
@@ -707,7 +707,7 @@ Section WpSconfLock.
     iPoseProof "Hhw" as "#Hhwc".
     iDestruct "Hhwc" as (misa0 mseccfg0 pmar0 elp0)
       "(#Hmisa & #Hmseccfg & #Hpma & #Hhtif & #Help & %HmisaS & %HmisaC &
-        %HmisaU & %HmisaM & %Hpma_all & %Hseccfg1 & %Hseccfg2 & %Help_np & %HmisaA & %Hmisa_val0 & %Hmseccfg_val0)".
+        %HmisaU & %HmisaM & %Hpma_all & %Hseccfg1 & %Hseccfg2 & %Help_np & %HmisaA & %Hmisa_val0 & %Hmseccfg_val0 & #Hkmapb)".
     destruct (Hpma_all pa 4) as (region_amo & Hmatch_amo & _ & Hread_amo & Hwrite_amo & Hatomic_supp_amo).
     assert (Hatomic_amo : pma_allows_atomic_op
               ((override_PMA (PMA_Region_attributes region_amo) PBMT_PMA).(PMA_atomic_support))
