iris/WpSconfMem.v
@@ -146,7 +146,7 @@ Section WpSconfMem.
     iPoseProof "Hhw" as "#Hhwc".
     iDestruct "Hhwc" as (misa0 mseccfg0 pmar0 elp0)
       "(#Hmisa & #Hmseccfg & #Hpma & #Hhtif & #Help & %HmisaS & %HmisaC &
-        %HmisaU & %HmisaM & %Hpma_all & %Hseccfg1 & %Hseccfg2 & %Help_np & %HmisaA & %Hmisa_val0 & %Hmseccfg_val0)".
+        %HmisaU & %HmisaM & %Hpma_all & %Hseccfg1 & %Hseccfg2 & %Help_np & %HmisaA & %Hmisa_val0 & %Hmseccfg_val0 & #Hkmapb)".
     destruct (Hpma_all pa width) as (region_ld & Hmatch_ld0 & _ & Hread_ld & _).
     iDestruct "Hsi" as "[Hreg [Hmem Hdev]]".
     iDestruct (reg_valid    with "Hreg Hpriv") as %Lpriv.
@@ -468,7 +468,7 @@ Section WpSconfMem.
     iPoseProof "Hhw" as "#Hhwc".
     iDestruct "Hhwc" as (misa0 mseccfg0 pmar0 elp0)
       "(#Hmisa & #Hmseccfg & #Hpma & #Hhtif & #Help & %HmisaS & %HmisaC &
-        %HmisaU & %HmisaM & %Hpma_all & %Hseccfg1 & %Hseccfg2 & %Help_np & %HmisaA & %Hmisa_val0 & %Hmseccfg_val0)".
+        %HmisaU & %HmisaM & %Hpma_all & %Hseccfg1 & %Hseccfg2 & %Help_np & %HmisaA & %Hmisa_val0 & %Hmseccfg_val0 & #Hkmapb)".
     destruct (Hpma_all pa width) as (region_st & Hmatch_st0 & _ & _ & Hwrite_st & _).
     iDestruct "Hsi" as "[Hreg [Hmem Hdev]]".
     iDestruct (reg_valid    with "Hreg Hpriv") as %Lpriv.
@@ -812,7 +812,7 @@ Section WpSconfMem.
     iPoseProof "Hhw" as "#Hhwc".
     iDestruct "Hhwc" as (misa0 mseccfg0 pmar0 elp0)
       "(#Hmisa & #Hmseccfg & #Hpma & #Hhtif & #Help & %HmisaS & %HmisaC &
-        %HmisaU & %HmisaM & %Hpma_all & %Hseccfg1 & %Hseccfg2 & %Help_np & %HmisaA & %Hmisa_val0 & %Hmseccfg_val0)".
+        %HmisaU & %HmisaM & %Hpma_all & %Hseccfg1 & %Hseccfg2 & %Help_np & %HmisaA & %Hmisa_val0 & %Hmseccfg_val0 & #Hkmapb)".
     destruct (Hpma_all pa 1) as (region_st & Hmatch_st0 & _ & _ & Hwrite_st & _).
     iDestruct "Hsi" as "[Hreg [Hmem Hdev]]".
     iDestruct (reg_valid    with "Hreg Hpriv") as %Lpriv.
@@ -1033,7 +1033,7 @@ Section WpSconfMem.
     iPoseProof "Hhw" as "#Hhwc".
     iDestruct "Hhwc" as (misa0 mseccfg0 pmar0 elp0)
       "(#Hmisa & #Hmseccfg & #Hpma & #Hhtif & #Help & %HmisaS & %HmisaC &
-        %HmisaU & %HmisaM & %Hpma_all & %Hseccfg1 & %Hseccfg2 & %Help_np & %HmisaA & %Hmisa_val0 & %Hmseccfg_val0)".
+        %HmisaU & %HmisaM & %Hpma_all & %Hseccfg1 & %Hseccfg2 & %Help_np & %HmisaA & %Hmisa_val0 & %Hmseccfg_val0 & #Hkmapb)".
     destruct (Hpma_all pa 8) as (region_st & Hmatch_st0 & _ & _ & Hwrite_st & _).
     iDestruct "Hsi" as "[Hreg [Hmem Hdev]]".
     iDestruct (reg_valid    with "Hreg Hpriv") as %Lpriv.
@@ -1213,7 +1213,7 @@ Section WpSconfMem.
     iPoseProof "Hhw" as "#Hhwc".
     iDestruct "Hhwc" as (misa0 mseccfg0 pmar0 elp0)
       "(#Hmisa & #Hmseccfg & #Hpma & #Hhtif & #Help & %HmisaS & %HmisaC &
-        %HmisaU & %HmisaM & %Hpma_all & %Hseccfg1 & %Hseccfg2 & %Help_np & %HmisaA & %Hmisa_val0 & %Hmseccfg_val0)".
+        %HmisaU & %HmisaM & %Hpma_all & %Hseccfg1 & %Hseccfg2 & %Help_np & %HmisaA & %Hmisa_val0 & %Hmseccfg_val0 & #Hkmapb)".
     destruct (Hpma_all pa 4) as (region_st & Hmatch_st0 & _ & _ & Hwrite_st & _).
     iDestruct "Hsi" as "[Hreg [Hmem Hdev]]".
     iDestruct (reg_valid    with "Hreg Hpriv") as %Lpriv.
