iris/WpSmodePtBtype.v
@@ -279,7 +279,7 @@ Section WpSmodePtBtype.
     iPoseProof "Hhw" as "#Hhwc".
     iDestruct "Hhwc" as (misa0 mseccfg0 pmar0 elp0)
       "(#Hmisa & #Hmseccfg & #Hpma & #Hhtif & #Help & %HmisaS & %HmisaC &
-        %HmisaU & %HmisaM & %Hpma_all & %Hseccfg1 & %Hseccfg2 & %Help_np & %HmisaA & %Hmisa_val0 & %Hmseccfg_val0)".
+        %HmisaU & %HmisaM & %Hpma_all & %Hseccfg1 & %Hseccfg2 & %Help_np & %HmisaA & %Hmisa_val0 & %Hmseccfg_val0 & #Hkmapb)".
     iApply (wp_instr_s_config_regime R Φ pc false (BTYPE (imm, Regidx rs2, Regidx rs1, BEQ))
               mstatus0 mie_v mdv0 menvcfg0
  HSIE HMPRV HSXL Hmm HPBMTE Hmenvval0
@@ -489,7 +489,7 @@ Section WpSmodePtBtype.
     iPoseProof "Hhw" as "#Hhwc".
     iDestruct "Hhwc" as (misa0 mseccfg0 pmar0 elp0)
       "(#Hmisa & #Hmseccfg & #Hpma & #Hhtif & #Help & %HmisaS & %HmisaC &
-        %HmisaU & %HmisaM & %Hpma_all & %Hseccfg1 & %Hseccfg2 & %Help_np & %HmisaA & %Hmisa_val0 & %Hmseccfg_val0)".
+        %HmisaU & %HmisaM & %Hpma_all & %Hseccfg1 & %Hseccfg2 & %Help_np & %HmisaA & %Hmisa_val0 & %Hmseccfg_val0 & #Hkmapb)".
     iApply (wp_instr_s_config_regime R Φ pc false (BTYPE (imm, Regidx rs2, Regidx rs1, BNE))
               mstatus0 mie_v mdv0 menvcfg0
  HSIE HMPRV HSXL Hmm HPBMTE Hmenvval0
