iris/WpSmodePtLeaves.v
@@ -422,7 +422,7 @@ Section WpSmodePtLoad.
     iPoseProof "Hhw" as "#Hhwc".
     iDestruct "Hhwc" as (misa0 mseccfg0 pmar0 elp0)
       "(#Hmisa & #Hmseccfg & #Hpma & #Hhtif & #Help & %HmisaS & %HmisaC &
-        %HmisaU & %HmisaM & %Hpma_all & %Hseccfg1 & %Hseccfg2 & %Help_np & %HmisaA & %Hmisa_val0 & %Hmseccfg_val0)".
+        %HmisaU & %HmisaM & %Hpma_all & %Hseccfg1 & %Hseccfg2 & %Help_np & %HmisaA & %Hmisa_val0 & %Hmseccfg_val0 & #Hkmapb)".
     destruct (Hpma_all pa 8) as (region_ld & Hmatch_ld0 & _ & Hread_ld & _).
     iApply (wp_instr_s_config_regime R Φ pc true (LOAD (imm, Regidx rs1, Regidx rd, false, 8))
               mstatus0 mie_v mdv0 menvcfg0
@@ -852,7 +852,7 @@ Section WpSmodePtStore.
     iPoseProof "Hhw" as "#Hhwc".
     iDestruct "Hhwc" as (misa0 mseccfg0 pmar0 elp0)
       "(#Hmisa & #Hmseccfg & #Hpma & #Hhtif & #Help & %HmisaS & %HmisaC &
-        %HmisaU & %HmisaM & %Hpma_all & %Hseccfg1 & %Hseccfg2 & %Help_np & %HmisaA & %Hmisa_val0 & %Hmseccfg_val0)".
+        %HmisaU & %HmisaM & %Hpma_all & %Hseccfg1 & %Hseccfg2 & %Help_np & %HmisaA & %Hmisa_val0 & %Hmseccfg_val0 & #Hkmapb)".
     destruct (Hpma_all pa 8) as (region_st & Hmatch_st0 & _ & _ & Hwrite_st & _).
     iApply (wp_instr_s_config_regime R Φ pc true (STORE (imm, Regidx rs2, Regidx rs1, 8))
               mstatus0 mie_v mdv0 menvcfg0
